PolyFun/PFunctor/Display/Handler.lean
@@ -318,7 +318,8 @@ theorem liftM_comp
     (dfirst : Handler S T first)
     (second : (a : Q.A) → FreeM R (Q.B a))
     (dsecond : Handler T U second) :
-    U.transport F (FreeM.liftM_comp (P := P) (Q := Q) (R := R) t first second)
+    U.transport F
+        (FreeM.liftM_comp (P := P) (Q := Q) (m := FreeM R) t first second)
         (T.liftM U (t.liftM first) (S.liftM T t d first dfirst)
           second dsecond) =
       S.liftM U t d (fun a => (first a).liftM second)
@@ -441,7 +442,7 @@ theorem comp_assoc_apply
     (first : Handler S T f) (second : Handler T U g)
     (third : Handler U W h) (a : P.A) (c : S.position a) :
     W.transport (S.direction a c)
-        (FreeM.liftM_comp (P := Q) (Q := R) (R := V) (f a) g h)
+        (FreeM.liftM_comp (P := Q) (Q := R) (m := FreeM V) (f a) g h)
         (third.comp (second.comp first) a c) =
       (third.comp second).comp first a c :=
   T.liftM_comp U W (f a) (first a c) g second h third
